theories/algebra/Counting.ec
@@ -1,0 +1,248 @@
+(* ==================================================================== *)
+require import AllCore Ring List Int IntMin IntDiv Bigalg Binomial Finite Poly StdBigop.
+(*---*) import StdOrder.IntOrder IntID Bigint.BIA.
+
+
+(* ==================================================================== *)
+(*TODO: surely some of this is done elsewhere, and move where appropriate.*)
+lemma le_ind P (m : int) :
+  P m =>
+  (forall n , m <= n => P n => P (n + 1)) =>
+  (forall n , m <= n => P n).
+proof.
+  move => Pm IH n /subr_ge0 le0_; rewrite -(subrK n m).
+  elim: (n - m) le0_ => {n} [|n le0n IHn] //.
+  by rewrite addrAC; apply/IH => //; apply/ler_addr.
+qed.
+
+lemma lt_ind P (m : int) :
+  P (m + 1) =>
+  (forall n , m < n => P n => P (n + 1)) =>
+  (forall n , m < n => P n).
+proof. by move => P_ IH n /ltzE; apply/le_ind => // {n} n /ltzE; apply/IH. qed.
+
+lemma strong_ind P :
+  P 0 =>
+  (forall n , (forall k , k \in range 0 n => P k) => P n) =>
+  (forall n , 0 <= n => P n).
+proof.
+  move => P0 IHS n le0n; elim: n le0n {1 2 4}n (le0n) (lerr n) => [|n le0n IHn] k.
+  + by move => le0k lek0; move: (eqz_leq k 0); rewrite lek0 le0k /= => ->>.
+  move => le0k /ler_eqVlt [->> {le0k}|/ltzS]; [|by apply/IHn].
+  by apply/IHS => k /mem_range [le0k /ltzS lekn]; apply/IHn.
+qed.
+
+lemma le_strong_ind P (m : int) :
+  P m =>
+  (forall n , (forall k , k \in range m n => P k) => P n) =>
+  (forall n , m <= n => P n).
+proof.
+  move => Pm IH n /subr_ge0 le0_; rewrite -(subrK n m).
+  move: (n - m) le0_ => +; move => {n} n le0n.
+  pose Q n:= P (n + m); apply/(strong_ind Q) => //.
+  move => {n le0n} n IHn; rewrite /(Q _); apply/IH.
+  move => k mem_; rewrite -(subrK k m); apply/IHn.
+  by apply/mem_range_subr.
+qed.
+
+lemma lt_strong_ind P (m : int) :
+  P (m + 1) =>
+  (forall n , (forall k , k \in range (m + 1) n => P k) => P n) =>
+  (forall n , m < n => P n).
+proof. by move => P_ IH n /ltzE; apply/le_strong_ind. qed.
+
+lemma add_ind P :
+  P 1 =>
+  (forall m n , 0 < m => 0 < n => P m => P n => P (m + n)) =>
+  (forall n , 0 < n => P n).
+proof. by move => P1 IHA; apply/lt_ind => // n lt0n Pn; apply/IHA. qed.
+
+(*TODO: move*)
+lemma prime2 :
+  prime 2.
+proof. by apply/primeP => /=; rewrite range_ltn // range_geq. qed.
+
+lemma compositeP n :
+  1 < n =>
+  ! prime n =>
+  exists a b , 1 < a /\ 1 < b /\ n = a * b.
+proof.
+  move => lt1n; apply/contraR; rewrite negb_exists /= => forall_.
+  apply/primeP; split => // a mem_; rewrite /coprime eq_sym.
+  apply/gcd_uniq => //=; [by rewrite negb_and gtr_eqF // ltzE ltzW|].
+  move => y /dvdzP [x] ->> dvdya; move/(_ x): forall_.
+  rewrite negb_exists /= => /(_ y) /= /negb_and; rewrite -!lerNgt.
+  case => //; apply/contraLR; rewrite -!ltrNge.
+  (*TODO: issue here*)
+  admit.
+qed.
+
+lemma mul_ind P :
+  (forall p , prime p => P p) =>
+  (forall m n , 1 < m => 1 < n => P m => P n => P (m * n)) =>
+  (forall n , 1 < n => P n).
+proof.
+  move => Pp IHM; apply/lt_strong_ind => /=.
+  + by apply/Pp/prime2.
+  move => n IHn; case: (prime n) => [prime_n|Nprime_n]; [by apply/Pp|].
+  search _ (!prime _).
+  admit.
+qed.
+
+lemma coprime_ind P :
+  (forall p n , prime p => 0 < n => P (p ^ n)) =>
+  (forall m n , 1 < m => 1 < n => coprime m n => P m => P n => P (m * n)) =>
+  (forall n , 1 < n => P n).
+proof.
+  admit.
+qed.
+
+
+(* ==================================================================== *)
+op coprimes n = filter (coprime n) (range 1 n).
+
+lemma coprimesP n k :
+  k \in coprimes n <=> (coprime n k /\ k \in range 1 n).
+proof. by rewrite mem_filter. qed.
+
+lemma coprimes_nil n :
+  n <= 1 =>
+  coprimes n = [].
+proof. by move => ?; rewrite /coprimes range_geq. qed.
+
+lemma coprimes1 n :
+  1 < n <=> 1 \in coprimes n.
+proof. by rewrite coprimesP /coprime gcdz1 /= mem_range. qed.
+
+lemma coprimes_prime p :
+  prime p =>
+  coprimes p = range 1 p.
+proof. by move => /primeP [lt1p mem_]; rewrite /coprimes eq_in_filter_predT. qed.
+
+lemma coprimes_pow_prime p n :
+  prime p =>
+  0 <= n =>
+  coprimes (p ^ (n + 1)) = flatten (mkseq (fun k => map (Int.(+) k) (coprimes (p ^ n))) p).
+proof.
+  move => prime_p le0n.
+  admit.
+qed.
+
+(* ------------------------------------------------------------------- *)
+op phi n = size (coprimes n).
+
+lemma phi_ge0 n :
+  0 <= phi n.
+proof. by apply/size_ge0. qed.
+
+lemma phi_eq0 n :
+  n <= 1 =>
+  phi n = 0.
+proof. by move => len0; rewrite /phi coprimes_nil. qed.
+
+lemma phi_gt0 n :
+  1 < n =>
+  0 < phi n.
+proof. by rewrite /phi -has_predT hasP => /coprimes1 ?; exists 1; rewrite /predT. qed.
+
+lemma phi_ltid n :
+  0 < n =>
+  phi n < n.
+proof.
+move => le0n; rewrite /phi /coprimes; apply/(ler_lt_trans (size (range 1 n))).
++ by apply/le_size_filter.
+by rewrite size_range ler_maxr; [rewrite -ltzS|rewrite ltzE].
+qed.
+
+lemma phi_prime p :
+  prime p =>
+  phi p = p - 1.
+proof.
+rewrite /phi => prime_p; move/coprimes_prime: (prime_p) => ->.
+by rewrite size_range maxrE subr_le0 lerNgt gt1_prime.
+qed.
+
+lemma phi_pow_prime p n :
+  prime p =>
+  0 < n =>
+  phi (p ^ n) = p ^ n - p ^ (n - 1).
+proof.
+  admit.
+qed.
+
+lemma phi_coprime m n :
+  0 < m =>
+  0 < n =>
+  phi (m * n) = phi m * phi n.
+proof.
+  admit.
+qed.
+
+(* ==================================================================== *)
+op divisors n = filter (transpose (%|) n) (range 1 (n + 1)).
+
+lemma divisors_nil n :
+  n <= 0 =>
+  divisors n = [].
+proof. by move => len0; rewrite /divisors range_geq // -ler_subr_addr. qed.
+
+lemma divisors_mem n :
+  0 < n =>
+  n \in divisors n.
+proof. by move => lt0n; rewrite /divisors rangeSr ?filter_rcons /= ?dvdzz /= ?mem_rcons //; move/ltzE: lt0n. qed.
+
+lemma divisors1 :
+  divisors 1 = [1].
+proof. by rewrite /divisors range_ltn // range_geq. qed.
+
+lemma divisors_prime p :
+  prime p =>
+  divisors p = [1; p].
+proof.
+  move => prime_p; rewrite /divisors rangeSr; [by move/ltzE: (gt0_prime _ prime_p)|].
+  rewrite filter_rcons /= dvdzz /= -cats1 -(cat1s 1); congr.
+  rewrite range_ltn ?gt1_prime //= dvd1z /=; apply/eq_in_filter_pred0 => k mem_ /=.
+  case/primeP: prime_p => _ /(_ k _); [by move: mem_; apply/mem_range_incl|].
+  rewrite /coprime => eq_1; apply/negP => /dvdzP [q] ->>; move: eq_1.
+  by rewrite gcdC gcdMl => /eqr_norml [[|] ->>]; move: mem_; rewrite mem_range.
+qed.
+
+lemma divisors_pow_prime p n :
+  prime p =>
+  0 <= n =>
+  divisors (p ^ n) = map (exp p) (range 0 n).
+proof.
+  admit.
+qed.
+
+lemma divisors_coprime m n :
+  0 < m =>
+  0 < n =>
+  coprime m n =>
+  perm_eq (divisors (m * n)) (allpairs Int.( * ) (divisors m) (divisors n)).
+proof.
+  admit.
+qed.
+
+lemma sum_phi n :
+  0 < n =>
+  big predT phi (divisors n) = n - 1.
+proof.
+  case/ltzE/ler_eqVlt => [<<-|/=]; [by rewrite divisors1 big_seq1 phi_eq0|].
+  pose P n:= big predT phi (divisors n) = n - 1; apply/(coprime_ind P); rewrite /P => {P}.
+  + move => p k prime_p lt0k; rewrite divisors_pow_prime ?ltzW // big_mapT.
+    rewrite big_ltn // {1}/(\o) expr0 phi_eq0 //=.
+    rewrite (eq_big_int _ _ _ (fun n => p ^ n - p ^ (n - 1))).
+    - by move => ? [?] _; rewrite /(\o) /= phi_pow_prime // ltzE.
+    rewrite -sumrB; move: (range_add 0 (k - 1) 1) => /= {2}->.
+    rewrite big_mapT (eq_big_int 0 _ _ ((^) p)); [by move => ?|].
+    case/ltzE/ler_eqVlt: lt0k => [<<-/=|/= lt1k].
+    - rewrite !big_geq // expr1.
+      admit.
+    rewrite (big_ltn 0) ?ltzS ?subr_gt0 // expr0 opprD addrA addrAC /=.
+    move: (rangeSr 1 (k - 1) _) => /=; [by apply/ltzS|move => ->].
+    rewrite big_rcons {1}/predT /= (addrAC _ (p ^ _)) /=.
+    search _ (_ _ + big _ _ (range _ _)).
+    admit.
+  admit.
+qed.
